verif_curve448Red.v
@@ -12,22 +12,24 @@ Local Open Scope Z.
 
 
 Definition prime: Z := 2^448 - 2^224 - 1.
+About list_repeat. 
+Definition undef14 := [Vundef;Vundef;Vundef;Vundef;Vundef;Vundef;Vundef;Vundef;Vundef;Vundef;Vundef;Vundef;Vundef;Vundef].
 
 Definition curve448Red_spec : ident * funspec :=
 DECLARE _curve448Red
 WITH    r : val,
         shr : share,
-        contents_r : list val,   
         a : val,
         contents_a : list Z,
         h : Z, (* may need writable share *)
         gv : globals
 PRE [ tptr tuint, tptr tuint, tuint ]
     PROP   (writable_share shr;
-            Zlength contents_r = 14;
-            Zlength contents_a = 14)
+            Zlength contents_a = 14;
+            0 <= (list_to_int contents_a) < (2 * prime)
+            (*TODO  * @param[in] h The highest term of A*))
     PARAMS (r ; a ; Vint(Int.repr h)) GLOBALS (gv)
-    SEP    (data_at shr (tarray tuint 14) contents_r r;
+    SEP    (data_at_ shr (tarray tuint 14) r;
             data_at Tsh (tarray tuint 14) (map Vint (map Int.repr contents_a)) a)
 POST [ tvoid ]
     PROP   ()
@@ -37,17 +39,21 @@ POST [ tvoid ]
             data_at Tsh (tarray tuint 14) (map Vint (map Int.repr contents_a)) a).
 
 Definition curve448Red_INV_1    (a : val)  (contents_a : list Z) 
-                                (b : val) (contents_b : list val) (shb : share)
+                                (b : val)  (r : val) (shr : share)
                                 (h : Z) (gv : globals) 
 := 
     (EX i : Z,
-    (PROP   (Zlength contents_a = 14;
-            writable_share shb)
+    (PROP   (Zlength contents_a = 14)
     LOCAL   (temp _temp (Vlong (Int64.repr (Int.signed (Int.repr 1))));
             lvar _b (tarray tuint 14) b; gvars gv; 
             temp _a a; temp _h (Vint (Int.repr h)))
-    SEP     (data_at shb (tarray tuint 14) 
-            (map Vint (map Int.repr contents_a)) a
+    SEP     ( 
+                data_at_ shr (tarray tuint 14) r;
+                data_at Tsh (tarray tuint 14) (map Vint (map Int.repr contents_a)) a; 
+                data_at Tsh (tarray tuint 14)  
+                ((sublist.sublist 0 i (map Vint (map Int.repr (int_to_list ((list_to_int contents_a) mod prime)))))
+                ++ sublist.sublist i 14 undef14)
+             b
             )))%assert.
                 
 Definition Gprog : funspecs := ltac:(with_library prog [ curve448Red_spec ]).
@@ -56,10 +62,13 @@ Lemma body_curve448Red : semax_body Vprog Gprog f_curve448Red curve448Red_spec.
 Proof.
     start_function.
     forward.
-    forward.
     forward_for_simple_bound 7 
-        (curve448Red_INV_1 a contents_a v_b contents_b shb h gv).  
-
-
-
-
+        (curve448Red_INV_1 a contents_a v_b r shr h gv).
+    entailer!.
+    autorewrite with sublist.
+    apply derives_refl.
+    try repeat forward.
+    entailer!.
+    unfold Int64.shru.
+     
+    rewrite functional_extensionality. 
